Defined firt three lemmas

formalization/Formalization/Syntax.lean
@@ -1,13 +1,44 @@
+namespace LambdaE
 
-/-!
-# ENVCAP Language
+inductive Typ where
+  | int  : Typ
+  | top  : Typ
+  | arr  : Typ → Typ → Typ
+  | and  : Typ → Typ → Typ
+  | rcd  : String → Typ → Typ
+  deriving Repr
 
-This module defines the syntax of the ENVCAP calculus.
--/
+inductive Op where
+  | app
+  | box
+  | mrg
+  deriving Repr
+
+inductive Exp where
+  | ctx    : Exp
+  | lit    : Nat → Exp
+  | unit   : Exp
+  | binop  : Op → Exp → Exp → Exp
+  | lam    : Typ → Exp → Exp
+  | proj   : Exp → Nat → Exp
+  | clos   : Exp → Typ → Exp → Exp
+  | lrec   : String → Exp → Exp
+  | rproj  : Exp → String → Exp
+  deriving Repr
+
+inductive IndexLookup : Typ -> Nat → Typ → Prop 
+| zero (A B : Typ) : IndexLookup (Typ.and A B) 0 B
+| succ (A B : Typ) (n : Nat) (C : Typ) : IndexLookup A n C → IndexLookup (Typ.and A B) (Nat.succ n) C
+
+inductive LabelIn : String -> Typ -> Prop
+| rcd (label : String) (T : Typ) : LabelIn label (Typ.rcd label T)
+| andl (A B : Typ) (label : String) : LabelIn label A → LabelIn label (Typ.and A B)
+| andr (A B : Typ) (label : String) : LabelIn label B → LabelIn label (Typ.and A B)
+
+end LambdaE
 
 namespace ENVCAP
 
-/-- Types in the ENVCAP language. -/
 inductive Typ where
   | int  : Typ
   | top  : Typ
@@ -17,7 +48,6 @@ inductive Typ where
   | sig  : Typ → Typ → Typ
   deriving Repr
 
-/-- Binary operators in the ENVCAP language. -/
 inductive Op where
   | app
   | withE
@@ -26,7 +56,6 @@ inductive Op where
   | mapp
   deriving Repr
 
-/-- Expressions in the ENVCAP language. -/
 inductive Exp where
   | ctx    : Exp
   | unit   : Exp
@@ -36,54 +65,83 @@ inductive Exp where
   | proj   : Exp → Nat → Exp
   | clos   : Exp → Typ → Exp → Exp
   | struct : Typ → Exp → Exp
-  | lrec    : String → Exp → Exp
+  | lrec   : String → Exp → Exp
   | rproj  : Exp → String → Exp
-  | slet    : Exp → Typ → Exp → Exp
-  | sopen   : Exp → Exp → Exp
+  | slet   : Exp → Typ → Exp → Exp
+  | sopen  : Exp → Exp → Exp
   deriving Repr
 
+inductive IndexLookup : Typ → Nat → Typ → Prop
+| zero (A B : Typ) : IndexLookup (Typ.and A B) 0 B
+| succ (A B : Typ) (n : Nat) (C : Typ) : IndexLookup A n C → IndexLookup (Typ.and A B) (Nat.succ n) C
+
+def ElaborateType : Typ → LambdaE.Typ
+  | Typ.int        => LambdaE.Typ.int
+  | Typ.top        => LambdaE.Typ.top
+  | Typ.arr t1 t2  => LambdaE.Typ.arr (ElaborateType t1) (ElaborateType t2)
+  | Typ.and t1 t2  => LambdaE.Typ.and (ElaborateType t1) (ElaborateType t2)
+  | Typ.rcd str t  => LambdaE.Typ.rcd str (ElaborateType t)
+  | Typ.sig t1 t2  => LambdaE.Typ.arr (ElaborateType t1) (ElaborateType t2)
+
+inductive LabelIn : String -> Typ -> Prop
+| rcd (label : String) (T : Typ) : LabelIn label (Typ.rcd label T)
+| andl (A B : Typ) (label : String) : LabelIn label A → LabelIn label (Typ.and A B)
+| andr (A B : Typ) (label : String) : LabelIn label B → LabelIn label (Typ.and A B)
 end ENVCAP
 
-/-!
-# LambdaE Calculus
+theorem TypeElaborationUniqueness : ∀ (srcT : ENVCAP.Typ) (dstT1 dstT2 : LambdaE.Typ),
+    ENVCAP.ElaborateType srcT = dstT1 →
+    ENVCAP.ElaborateType srcT = dstT2 →
+    dstT1 = dstT2 := by 
+  intro srcT dstT1 dstT2 h1 h2;
+  rw [← h1];
+  rw [← h2];
 
-This module defines the syntax of the λE calculus.
--/
-namespace LambdaE
-
-/--
-Types in the λE calculus.
--/
-inductive Typ where
-  | int  : Typ
-  | top  : Typ
-  | arr  : Typ → Typ → Typ
-  | and  : Typ → Typ → Typ
-  | rcd  : String → Typ → Typ
-  deriving Repr
-
-/--
-Binary operators in λE.
--/
-inductive Op where
-  | app
-  | box
-  | mrg
-  deriving Repr
-
-/--
-Expressions in the λE.
--/
-inductive Exp where
-  | ctx    : Exp
-  | lit    : Nat → Exp
-  | unit   : Exp
-  | binop  : Op → Exp → Exp → Exp
-  | lam    : Typ → Exp → Exp
-  | proj   : Exp → Nat → Exp
-  | clos   : Exp → Typ → Exp → Exp
-  | lrec    : String → Exp → Exp
-  | rproj  : Exp → String → Exp
-  deriving Repr
-
-end LambdaE
+theorem TypeSafeIndexLookup : ∀ (srcT1 : ENVCAP.Typ) (n : Nat) (srcT2 : ENVCAP.Typ),
+    ENVCAP.IndexLookup srcT1 n srcT2 → 
+    LambdaE.IndexLookup (ENVCAP.ElaborateType srcT1) n (ENVCAP.ElaborateType srcT2) := by
+      intro srcT1 n srcT2 H;
+      induction H with
+      | zero A B =>
+          apply LambdaE.IndexLookup.zero;
+      | succ A B n C _ IH =>
+          rw [ENVCAP.ElaborateType];
+          apply LambdaE.IndexLookup.succ;  
+          apply IH;
+        
+theorem TypeSafeLabelIn : ∀ (label : String) (srcT : ENVCAP.Typ),
+    ENVCAP.LabelIn label srcT ↔ 
+    LambdaE.LabelIn label (ENVCAP.ElaborateType srcT) := by
+      intro label srcT;
+      apply Iff.intro;
+      · intro H;
+        induction H with
+        | rcd label T =>
+            rw [ENVCAP.ElaborateType];
+            apply LambdaE.LabelIn.rcd;
+        | andl A B label _ IH =>
+            rw [ENVCAP.ElaborateType];
+            apply LambdaE.LabelIn.andl;
+            apply IH;
+        | andr A B label _ IH =>
+            rw [ENVCAP.ElaborateType];
+            apply LambdaE.LabelIn.andr;
+            apply IH;
+      · intro H;
+        induction srcT with
+        | rcd labelA T IH => 
+            rw [ENVCAP.ElaborateType] at H;
+            cases H
+            apply ENVCAP.LabelIn.rcd
+        | and A B IH1 IH2 => 
+            rw [ENVCAP.ElaborateType] at H;
+            cases H with
+            | andl _ _ _ H1 =>
+                apply ENVCAP.LabelIn.andl;
+                apply IH1;
+                apply H1;
+            | andr _ _ _ H2 =>
+                apply ENVCAP.LabelIn.andr;
+                apply IH2;
+                apply H2;
+        | _ => cases H
